examples/low-level/crypto/Crypto.Symmetric.GF128.fst
@@ -7,17 +7,35 @@ open FStar.UInt8
 open FStar.Int.Cast
 open FStar.Buffer
 
-open Crypto.Symmetric.Bytes
-open Crypto.Symmetric.GF128.Spec
-
 module U32 = FStar.UInt32
+module U128 = FStar.UInt128
 module Spec = Crypto.Symmetric.GF128.Spec
-
+open Spec
 
 let len = 16ul // length of GF128 in bytes
 
 type elem = Spec.elem 
-type elemB = b:lbuffer 16
+type elemB = b:buffer U128.t{length b = 1}
+
+let load128_le b = 
+    let b1 = sub b 0ul 8ul in
+    let b2 = sub b 8ul 8ul in
+    let l1 = C.load64_le b1 in
+    let i1 = uint64_to_uint128 l1 in
+    let l2 = C.load64_le b2 in
+    let i2 = uint64_to_uint128 l2 in
+    let b = U128.(i2 <<^ 64ul) in
+    U128.(b +^ i1)
+
+
+let store128_le b i = 
+    let b1 = sub b 0ul 8ul in
+    let b2 = sub b 8ul 8ul in
+    let i1 = uint128_to_uint64 (U128.(i >>^ 64ul)) in
+    let i2 = uint128_to_uint64 i in
+    C.store64_le b1 i2;
+    C.store64_le b2 i1
+
 
 (* * Every block of message is regarded as an element in Galois field GF(2^128), **)
 (* * it is represented as 16 bytes. The following several functions are basic    **)
@@ -28,118 +46,86 @@ type elemB = b:lbuffer 16
 
 //16-09-23 we still miss a math specification of GF128 and a correctness proof.
 
-(* Every function "func_name_loop" is a helper for function "func_name". *)
-
-private val gf128_add_loop: 
-  a:elemB -> b:elemB {disjoint a b} ->
-  dep:u32{U32.(dep <=^ len)} -> Stack unit
-  (requires (fun h -> live h a /\ live h b))
-  (ensures  (fun h0 _ h1 -> live h0 a /\ live h0 b /\ live h1 a /\ modifies_1 a h0 h1))
-let rec gf128_add_loop a b dep =
-  if dep = 0ul then ()
-  else
-    let i = U32.(dep -^ 1ul) in
-    gf128_add_loop a b i;
-    a.(i) <- a.(i) ^^ b.(i)
-
 (* In place addition. Calculate "a + b" and store the result in a. *)
 val gf128_add: a:elemB -> b:elemB {disjoint a b} -> Stack unit
   (requires (fun h -> live h a /\ live h b))
   (ensures (fun h0 _ h1 -> 
-    live h0 a /\ live h0 b /\ live h1 a /\ modifies_1 a h0 h1 /\ 
-    as_seq h1 a == as_seq h0 a +@ as_seq h0 b))
+    live h0 a /\ live h0 b /\ live h1 a /\ modifies_1 a h0 h1))
 let gf128_add a b = 
-  let h0 = ST.get() in
-  gf128_add_loop a b len;
-  let h1 = ST.get() in
-  assume (as_seq h1 a == as_seq h0 a +@ as_seq h0 b)
-  //16-10-27 TODO: functional correctness.
-
-  
-private val gf128_shift_right_loop: a:elemB -> dep:u32{U32.(dep <^ len)} -> Stack unit
-  (requires (fun h -> live h a))
-  (ensures (fun h0 _ h1 -> live h1 a /\ modifies_1 a h0 h1))
-let rec gf128_shift_right_loop a dep =
-  if dep = 0ul 
-  then a.(0ul) <- shift_right a.(0ul) 1ul
-  else begin
-    let i = U32.(dep -^ 1ul) in
-    a.(dep) <- (a.(i) <<^ 7ul) +%^ (a.(dep) >>^ 1ul);
-    gf128_shift_right_loop a i
-  end
+  let av = a.(0ul) in
+  let bv = b.(0ul) in
+  let r = U128.(av ^^ bv) in
+  a.(0ul) <- r 
 
 (* In place shift. Calculate "a >> 1" and store the result in a. *)
 private val gf128_shift_right: a:elemB -> Stack unit
   (requires (fun h -> live h a))
   (ensures (fun h0 _ h1 -> live h1 a /\ modifies_1 a h0 h1))
-let gf128_shift_right a = gf128_shift_right_loop a 15ul
+let gf128_shift_right a = 
+  let av = a.(0ul) in
+  let a' = U128.(av >>^ 1ul) in
+  a.(0ul) <- a'
+
+
+let one_128 = uint64_to_uint128(1uL)
+let zero_128 = uint64_to_uint128(0uL)
+private let r_mul = U128.(uint64_to_uint128(225uL) <<^ 120ul)
 
 (* Generate mask. If the i-th bit of num is 1 then return 11111111, otherwise return 00000000. *)
-private val ith_bit_mask: num:byte -> i:u32{U32.v i < 8} -> Tot byte
+private val ith_bit_mask: num:U128.t -> i:U32.t{U32.v i < 128} -> Tot U128.t
 let ith_bit_mask num i =
-  let proj = shift_right 128uy i in
-  let res = logand num proj in
-  eq_mask res proj
+  let mi = U32.(127ul -^ i) in
+  let proj = U128.(one_128 <<^ mi) in
+  let res = U128.(num &^ proj) in
+  U128.(eq_mask res proj)
 
-private val apply_mask_loop: a:elemB -> m:elemB {disjoint a m} -> msk:byte -> dep:u32{U32.v dep <= 16} -> Stack unit
-  (requires (fun h -> live h a /\ live h m))
-  (ensures (fun h0 _ h1 -> live h1 m /\ modifies_1 m h0 h1))
-let rec apply_mask_loop a m msk dep =
-  if dep <> 0ul then 
+private val zero_bit_mask: num:U128.t -> Tot U128.t
+let zero_bit_mask num =
+  let proj = U128.(one_128) in
+  let res = U128.(num &^ proj) in
+  U128.(eq_mask res proj)
+
+val gf128_mul_loop: 
+  x:elemB -> 
+  v:elemB {disjoint x v} -> 
+  z:elemB {disjoint x z /\ disjoint v z} ->
+  ctr:U32.t{U32.v ctr <= 128} -> 
+  Stack unit
+  (requires (fun h -> live h x /\ live h v /\ live h z))
+  (ensures (fun h0 _ h1 -> live h1 x /\ live h1 v /\ live h1 z /\ modifies_2 v z h0 h1))
+let rec gf128_mul_loop x v z ctr =
+  if ctr <> 128ul then 
   begin
-    let i = U32.(dep -^ 1ul) in
-    m.(i) <- a.(i) &^ msk;
-    apply_mask_loop a m msk i
-  end
+    let xv = x.(0ul) in
+    let vv = v.(0ul) in
+    let zv = z.(0ul) in
 
-(* This will apply a mask to each byte of bytes. *)
-(* Mask a with msk, and store the result in m. *)
-private val apply_mask: a:elemB -> m:elemB {disjoint a m} -> msk:byte -> Stack unit
-  (requires (fun h -> live h a /\ live h m))
-  (ensures (fun h0 _ h1 -> live h1 m /\ modifies_1 m h0 h1))
-let apply_mask a m msk = apply_mask_loop a m msk len
+    let mski = ith_bit_mask xv ctr in     
+    let msk_v = U128.(vv &^ mski) in
+    z.(0ul) <- U128.(zv ^^ msk_v);
 
-private let r_mul = 225uy
-
-private val gf128_mul_loop: 
-  a:elemB -> b:elemB {disjoint a b} -> tmp:buffer {length tmp = 32 /\ disjoint a tmp /\ disjoint b tmp} ->
-  dep:u32{U32.v dep <= 128} -> Stack unit
-  (requires (fun h -> live h a /\ live h b /\ live h tmp))
-  (ensures (fun h0 _ h1 -> live h1 a /\ live h1 tmp /\ modifies_2 a tmp h0 h1))
-let rec gf128_mul_loop a b tmp dep =
-  if dep <> 128ul then 
-  begin
-    let r = sub tmp 0ul len in
-    let m = sub tmp len len in
-    let num = b.(U32.(dep /^ 8ul)) in
-    let msk = ith_bit_mask num (U32.rem dep 8ul) in
-    apply_mask a m msk;
-    gf128_add r m;
-    let num = a.(15ul) in
-    let msk = ith_bit_mask num 7ul in
-    gf128_shift_right a;
-    let num = a.(0ul) in
-    a.(0ul) <- (num ^^ (logand msk r_mul));
-    gf128_mul_loop a b tmp (U32.(dep +^ 1ul))
+    let msk0 = zero_bit_mask vv in
+    let msk_r_mul = U128.(r_mul &^ msk0) in
+    gf128_shift_right v;
+    let vv = v.(0ul) in
+    v.(0ul) <- U128.(vv ^^ msk_r_mul);
+    gf128_mul_loop x v z (U32.(ctr +^ 1ul))
   end
 
 (* In place multiplication. Calculate "a * b" and store the result in a.    *)
 (* WARNING: may have issues with constant time. *)
-val gf128_mul: a:elemB -> b:elemB {disjoint a b} -> Stack unit
-  (requires (fun h -> live h a /\ live h b))
+val gf128_mul: x:elemB -> y:elemB {disjoint x y} -> Stack unit
+  (requires (fun h -> live h x /\ live h y))
   (ensures (fun h0 _ h1 -> 
-    live h0 a /\ live h0 b /\ live h1 a /\ modifies_1 a h0 h1 /\ 
-    as_seq h1 a == as_seq h0 a *@ as_seq h0 b ))
-let gf128_mul a b =
+    live h1 x /\ live h1 y /\ modifies_1 x h0 h1))
+let gf128_mul x y =
   let h0 = ST.get() in
   push_frame();
-  let tmp = create 0uy 32ul in
-  gf128_mul_loop a b tmp 0ul;
-  blit tmp 0ul a 0ul 16ul;
-  pop_frame();
-  let h1 = ST.get() in
-  assume(as_seq h1 a == as_seq h0 a *@ as_seq h0 b)
-  //16-10-27 todo: functional correctness.
+  let z = create zero_128 1ul in
+  gf128_mul_loop y x z 0ul;
+  x.(0ul) <- z.(0ul);
+  pop_frame()
+
 
 val add_and_multiply: acc:elemB -> block:elemB{disjoint acc block}
   -> k:elemB{disjoint acc k /\ disjoint block k} -> Stack unit
@@ -147,23 +133,25 @@ val add_and_multiply: acc:elemB -> block:elemB{disjoint acc block}
   (ensures (fun h0 _ h1 -> live h0 acc /\ live h0 block /\ live h0 k
     /\ live h1 acc /\ live h1 k
     /\ modifies_1 acc h0 h1
-    /\ as_seq h1 acc == (as_seq h0 acc +@ as_seq h0 block) *@ as_seq h0 k))
+    /\ get h1 acc 0 == (get h0 acc 0) +@ (get h0 block 0) *@ (get h0 k 0)))
 let add_and_multiply acc block k =
   gf128_add acc block;
   gf128_mul acc k
 
 
-val finish: acc:elemB -> s:elemB -> Stack unit
+val finish: acc:elemB -> s:buffer UInt8.t{length s = 16} -> Stack unit
   (requires (fun h -> live h acc /\ live h s /\ disjoint acc s))
   (ensures  (fun h0 _ h1 -> live h0 acc /\ live h0 s
     /\ modifies_1 acc h0 h1 /\ live h1 acc
-    /\ as_seq h1 acc == finish (as_seq h0 acc) (as_seq h0 s)))
+    /\ decode (get h1 acc 0) == finish (get h0 acc 0) (as_seq h0 s)))
 let finish a s = 
   //let _ = IO.debug_print_string "finish a=" in 
   //let _ = Crypto.Symmetric.Bytes.print_buffer a 0ul 16ul in
   //let _ = IO.debug_print_string "finish s=" in 
   //let _ = Crypto.Symmetric.Bytes.print_buffer s 0ul 16ul in
-  gf128_add a s
+  let sb = create zero_128 1ul in
+  sb.(0ul) <- load128_le s;
+  gf128_add a sb
   //let _ = IO.debug_print_string "finish a=" in 
   //let _ = Crypto.Symmetric.Bytes.print_buffer a 0ul 16ul in
 
@@ -176,71 +164,57 @@ let finish a s =
 private val ghash_loop_:
   tag:elemB ->
   auth_key:elemB {disjoint tag auth_key} ->
-  str:buffer{disjoint tag str /\ disjoint auth_key tag} ->
-  len:u32{length str = U32.v len} ->
-  dep:u32{U32.v dep <= U32.v len} -> Stack unit
+  str:buffer UInt8.t{disjoint tag str /\ disjoint auth_key tag} ->
+  tmp:buffer UInt128.t{disjoint tag tmp /\ disjoint auth_key tmp /\ disjoint str tmp} ->
+  len:U32.t{length str = U32.v len} ->
+  dep:U32.t{U32.v dep <= U32.v len} -> Stack unit
   (requires (fun h -> U32.v len - U32.v dep <= 16 /\ live h tag /\ live h auth_key /\ live h str))
   (ensures (fun h0 _ h1 -> live h1 tag /\ live h1 auth_key /\ live h1 str /\ modifies_1 tag h0 h1))
-let ghash_loop_ tag auth_key str len dep =
+let ghash_loop_ tag auth_key str tmp len dep =
   push_frame();
-  let last = create 0uy 16ul in
-  blit str dep last 0ul (U32.(len -^ dep)); 
-  add_and_multiply tag last auth_key;
+  let t = create 0uy 16ul in
+  blit str dep t 0ul (U32.(len -^ dep));
+  tmp.(0ul) <- load128_le t;
+  add_and_multiply tag tmp auth_key;
   pop_frame()
 
 (* WARNING: may have issues with constant time. *)
 private val ghash_loop: 
   tag:elemB ->
   auth_key:elemB {disjoint tag auth_key} ->
-  str:buffer{disjoint tag str /\ disjoint auth_key str} ->
-  len:u32{length str = U32.v len} ->
-  dep:u32{U32.v dep <= U32.v len} -> Stack unit
-  (requires (fun h -> live h tag /\ live h auth_key /\ live h str))
-  (ensures (fun h0 _ h1 -> live h1 tag /\ live h1 auth_key /\ live h1 str /\ modifies_1 tag h0 h1))
-let rec ghash_loop tag auth_key str len dep =
+  str:buffer UInt8.t{disjoint tag str /\ disjoint auth_key str} ->
+  tmp:buffer UInt128.t{disjoint tag tmp /\ disjoint auth_key tmp /\ disjoint str tmp} ->
+  len:U32.t{length str = U32.v len} ->
+  dep:U32.t{U32.v dep <= U32.v len} -> Stack unit
+  (requires (fun h -> live h tag /\ live h auth_key /\ live h str /\ live h tmp))
+  (ensures (fun h0 _ h1 -> live h1 tag /\ live h1 auth_key /\ live h1 str /\ live h1 tmp /\ modifies_2 tag tmp h0 h1))
+let rec ghash_loop tag auth_key str tmp len dep =
   (* Appending zeros if the last block is not complete *)
   let rest = U32.(len -^ dep) in 
   if rest <> 0ul then 
-  if U32.(16ul >=^ rest) then ghash_loop_ tag auth_key str len dep
+  if U32.(16ul >=^ rest) then ghash_loop_ tag auth_key str tmp len dep
   else 
   begin
     let next = U32.add dep 16ul in
     let si = sub str dep 16ul in
-    add_and_multiply tag si auth_key;
-    ghash_loop tag auth_key str len next
+    tmp.(0ul) <- load128_le si;
+    add_and_multiply tag tmp auth_key;
+    ghash_loop tag auth_key str tmp len next
   end
  
 (* During authentication, the length information should also be included. *)
 (* This function will generate an element in GF128 by:                    *)
 (* 1. express len of additional data and len of ciphertext as 64-bit int; *)
 (* 2. concatenate the two integers to get a 128-bit block.                *)
-private val mk_len_info: len_info:buffer{length len_info = 16} ->
-    len_1:u32 -> len_2:u32 -> Stack unit
+private val mk_len_info: len_info:elemB ->
+    len_1:U32.t -> len_2:U32.t -> Stack unit
     (requires (fun h -> live h len_info))
     (ensures (fun h0 _ h1 -> live h1 len_info /\ modifies_1 len_info h0 h1))
 let mk_len_info len_info len_1 len_2 =
-  let last = shift_left (uint32_to_uint8 len_1) 3ul in
-  let open FStar.UInt32 in
-  upd len_info 7ul last;
-  let len_1 = len_1 >>^ 5ul in
-  upd len_info 6ul (uint32_to_uint8 len_1);
-  let len_1 = len_1 >>^ 8ul in
-  upd len_info 5ul (uint32_to_uint8 len_1);
-  let len_1 = len_1 >>^ 8ul in
-  upd len_info 4ul (uint32_to_uint8 len_1);
-  let len_1 = len_1 >>^ 8ul in
-  upd len_info 3ul (uint32_to_uint8 len_1);
-  let last = FStar.UInt8.(uint32_to_uint8 len_2 <<^ 3ul) in
-  upd len_info 15ul last;
-  let len_2 = len_2 >>^ 5ul in
-  upd len_info 14ul (uint32_to_uint8 len_2);
-  let len_2 = len_2 >>^ 8ul in
-  upd len_info 13ul (uint32_to_uint8 len_2);
-  let len_2 = len_2 >>^ 8ul in
-  upd len_info 12ul (uint32_to_uint8 len_2);
-  let len_2 = len_2 >>^ 8ul in
-  upd len_info 11ul (uint32_to_uint8 len_2)
-// relying on outer initialization?
+  let l1 = uint64_to_uint128(uint32_to_uint64 len_1) in
+  let l2 = uint64_to_uint128(uint32_to_uint64 len_2) in
+  let u = U128.((l1 <<^ 64ul) +^ l2) in
+  len_info.(0ul) <- u
 
 #reset-options "--initial_fuel 0 --max_fuel 0 --z3rlimit 20"
 
@@ -248,10 +222,10 @@ let mk_len_info len_info len_1 len_2 =
 (* then ciphertext and at last length information. The result is stored in tag.        *)
 val ghash:
   k:elemB ->
-  ad:buffer{disjoint k ad} ->
-  adlen:u32{U32.v adlen = length ad} ->
-  ciphertext:buffer{disjoint k ciphertext /\ disjoint ad ciphertext} ->
-  len:u32{U32.v len = length ciphertext} ->
+  ad:buffer UInt8.t{disjoint k ad} ->
+  adlen:U32.t{U32.v adlen = length ad} ->
+  ciphertext:buffer UInt8.t{disjoint k ciphertext /\ disjoint ad ciphertext} ->
+  len:U32.t{U32.v len = length ciphertext} ->
   tag:elemB{disjoint k tag /\ disjoint ad tag /\ disjoint ciphertext tag} ->
   Stack unit
   (requires (fun h -> live h k /\ live h ad /\ live h ciphertext /\ live h tag))
@@ -260,13 +234,14 @@ val ghash:
 let ghash k ad adlen ciphertext len tag =
   push_frame();
   let h0 = ST.get() in
-  let len_info = create (0uy) 16ul in
+  let len_info = create zero_128 1ul in
   mk_len_info len_info adlen len;
   let h1 = ST.get() in
   assert(modifies_0 h0 h1);
-  fill tag 0uy 16ul;
-  ghash_loop tag k ad adlen 0ul;
-  ghash_loop tag k ciphertext len 0ul;
+  tag.(0ul) <- zero_128;
+  let tmp = create zero_128 1ul in
+  ghash_loop tag k ad tmp adlen 0ul;
+  ghash_loop tag k ciphertext tmp len 0ul;
   add_and_multiply tag len_info k;
   //gf128_add tag len_info;
   //gf128_mul tag k;
