examples/low-level/crypto/Crypto.Symmetric.MAC.Spec.fst
@@ -1,0 +1,90 @@
+module Crypto.Symmetric.MAC.Spec
+
+open Crypto.Symmetric.Bytes 
+open Crypto.Indexing
+module GS = Crypto.Symmetric.GF128.Spec
+module PS = Crypto.Symmetric.Poly1305.Spec
+
+let elem (a:macAlg) =
+  match a with 
+  | POLY1305 -> PS.elem
+  | GHASH    -> GS.elem
+
+let zero a : elem a = 
+  match a with 
+  | POLY1305 -> PS.zero
+  | GHASH    -> GS.zero
+
+
+let op_Plus_At (#a:macAlg) (e1:elem a) (e2:elem a) : Tot (elem a) =	
+  match a with
+  | POLY1305 -> PS.op_Plus_At e1 e2
+  | GHASH -> GS.op_Plus_At e1 e2
+
+let op_Star_At (#a:macAlg) (e1:elem a) (e2:elem a) : Tot (elem a) =	
+  match a with
+  | POLY1305 -> PS.op_Star_At e1 e2
+  | GHASH -> GS.op_Star_At e1 e2
+    
+type polynomial a = Seq.seq (elem a)
+
+val update: #a:macAlg -> r:elem a -> acc:elem a -> e:elem a -> Tot (acc':elem a)
+let update #a r acc e = 
+    (acc +@ e) *@ r
+
+(** Polynomial evaluation *)
+val poly_eval: #a:macAlg -> p:polynomial a -> r:elem a -> Tot (elem a) (decreases (Seq.length p))
+let rec poly_eval #a p r =
+    if Seq.length p = 0 then zero a
+    else 
+      let h = SeqProperties.head p in 
+      let t = SeqProperties.tail p in 
+      update #a r (poly_eval t r) h
+
+(** message words (not necessarily a full word. *)
+let wlen = 16ul
+type word = b:bytes{Seq.length b <= UInt32.v wlen}
+type word_16 = b:bytes{Seq.length b = UInt32.v wlen}
+
+(** Encode a word of a message as a field element *)
+val encode: #a:macAlg -> w:word_16 -> Tot (elem a)
+let encode #a w =
+  match a with 
+  | POLY1305 -> PS.encode w
+  | GHASH    -> GS.encode w
+
+
+type text = Seq.seq word_16
+val encode_text: #a:macAlg -> x:text -> Tot (polynomial a) (decreases (Seq.length x))
+let rec encode_text #a x =
+    if Seq.length x = 0 then Seq.createEmpty #(elem a)
+    else 
+      let h = SeqProperties.head x in 
+      let t = SeqProperties.tail x in 
+      SeqProperties.cons (encode #a h) (encode_text #a t)
+
+let taglen = 16ul
+type tag = word_16
+
+val decode: #a:macAlg -> e:elem a -> Tot (w:word_16)
+let decode #a e =
+  match a with 
+  | POLY1305 -> PS.decode e
+  | GHASH    -> GS.decode e
+
+
+val finish: #a:macAlg -> acc:elem a -> s:tag -> Tot tag
+let finish #a acc s = 
+  match a with 
+  | POLY1305 -> PS.finish acc s
+  | GHASH    -> GS.finish acc s
+
+
+val mac_poly: #a:macAlg -> x:text -> r: elem a -> s: tag -> Tot tag 
+let mac_poly #a x r s =
+    let p = encode_text #a x in
+    let v = poly_eval #a p r in
+    finish #a v s
+
+
+    
