examples/low-level/crypto/Crypto.Symmetric.UF1CMA.Spec.fst
@@ -1,0 +1,166 @@
+(**
+   This file states our probabilistic security assumption on
+   polynomial MACs, and provides an idealized implementation,
+   while being abstract on the underlying field.
+*)
+module Crypto.Symmetric.UF1CMA.Spec
+
+open Crypto.Symmetric.MAC.Spec
+open Crypto.Symmetric.Bytes
+open Crypto.Indexing
+open Flag
+
+open FStar.HyperHeap
+open FStar.HyperStack
+
+module HH = FStar.HyperHeap
+module HS = FStar.HyperStack
+module RR = FStar.Monotonic.RRef
+
+
+(** Authenticated payload: a sequence of words *)
+type text = Seq.seq word_16
+type tag  = tag
+
+(** One-time MAC log, None or Some (m, MAC(m)) *)
+type log = option (text * tag) 
+
+let log_cmp (a:log) (b:log) =
+  match a,b with
+  | Some (l,t) , Some (l',t') -> l == l' /\ t == t' // avoid inversion
+  | None, _                   -> True
+  | _                         -> False
+
+val log_cmp_monotonic: unit -> Lemma (RR.monotonic log log_cmp)
+let log_cmp_monotonic _ = ()
+
+let erid = r:HH.rid{HS.is_eternal_region r}
+
+let ideal_log (r:erid) = RR.m_rref r log log_cmp
+
+let log_ref (r:erid) = if mac_log then ideal_log r else unit
+
+let ilog (#r:erid) (l:log_ref r{mac_log}) : Tot (ideal_log r) = l
+
+type alg = macAlg
+
+let alg_of_id = macAlg_of_id
+
+noeq type state (i:id) =
+  | State:
+    #region: erid ->
+    r: elem (alg_of_id i) ->
+    s: word_16 ->
+    log: log_ref region ->
+    state i
+
+
+(** Length of the single-use part of the key *)
+let keylen (i:id) = 
+  match aeadAlg_of_id i with
+  | AES_128_GCM       -> 16ul
+  | AES_256_GCM       -> 16ul
+  | CHACHA20_POLY1305 -> 32ul
+
+(** Length of optional static auth key (when using AES) *)
+let skeylen (i:id) =  // can't refine with {skeyed i} here
+  match aeadAlg_of_id i with
+  | AES_128_GCM       -> 16ul
+  | AES_256_GCM       -> 16ul
+  | _                 ->  0ul // dummy; never allocated.
+
+(** Does the algorithm use a static key? *)
+let skeyed (i:id) = 
+  match aeadAlg_of_id i with
+  | AES_128_GCM       -> true
+  | AES_256_GCM       -> true
+  | CHACHA20_POLY1305 -> false
+
+type key (i:id) = b:bytes{Seq.length b = UInt32.v (keylen i)}
+type skey (i:id) = b:bytes{Seq.length b = UInt32.v (skeylen i)}
+type akey (i:id) = o:option (skey i){is_Some o <==> skeyed i}
+
+val get_skey: #i:id{skeyed i} -> akey i -> Tot (skey i)
+let get_skey #i (Some k) = k
+
+let genPost (i:id) (region:erid) m0 (st:state i) m1 =
+   st.region == region /\
+   (mac_log ==>
+      ~(RR.m_contains (ilog st.log) m0) /\
+      RR.m_contains (ilog st.log) m1 /\
+      RR.m_sel m1 (ilog st.log) == None)
+
+val alloc: region:erid -> i:id
+  -> ak:akey i
+  -> k: key i
+  -> ST (state i)
+  (requires (fun m0 -> true))
+  (ensures  (fun m0 st m1 -> genPost i region m0 st m1 /\ HS.modifies_one region m0 m1))
+let alloc region i ak k =
+  let (rb,sb):(lbytes 16 * lbytes 16) =
+    if skeyed i then
+      get_skey #i ak, k 
+    else
+       Seq.slice k 0 16, Seq.slice k 16 32
+  in
+  let r = encode rb in
+  let s:word_16 = sb in
+  if mac_log then
+    begin
+    log_cmp_monotonic ();
+    let log = RR.m_alloc #log #log_cmp region None in
+    State #i #region r s log
+    end
+  else
+    State #i #region r s ()
+
+val gen: region:erid -> i:id -> ak:akey i -> ST (state i)
+  (requires (fun m0 -> true))
+  (ensures (fun m0 st m1 -> genPost i region m0 st m1 /\ HS.modifies_one region m0 m1))
+let gen region i ak =
+  let len = keylen i in
+  let k = random_bytes len in
+  alloc region i ak k
+
+
+assume val authId: id -> Tot bool
+
+val coerce: region:erid -> i:id{~(authId i)}
+  -> ak:akey i
+  -> k:key i
+  -> ST (state i)
+  (requires (fun m0 -> true))
+  (ensures (fun m0 st m1 -> genPost i region m0 st m1 /\ HS.modifies_one region m0 m1))
+let coerce region i ak k =
+  alloc region i ak k
+
+let irtext = if mac_log then HS.reference text else unit
+
+noeq abstract type accBuffer (i:id) =
+  | Acc: a:elem (alg_of_id i) ->
+         l:irtext ->
+         accBuffer i
+
+let alog (#i:id) (acc:accBuffer i{mac_log}) : HS.reference text =
+  acc.l
+
+let acc_inv (#i:id) (st:state i) (acc:accBuffer i) h =
+  (mac_log ==> (
+    let log = HS.sel h (alog acc) in
+    let a = acc.a in
+    let r = st.r in
+    HS.contains h (alog acc) /\
+    a == poly_eval #(alg_of_id i) (encode_text log) r))
+
+
+val start: #i:id -> st:state i -> StackInline (accBuffer i)
+  (requires (fun h -> true))
+  (ensures  (fun h0 a h1 ->
+    acc_inv st a h1 /\ 
+    h0 = h1))
+
+let start #i st =
+  let t:text = Seq.createEmpty #word_16 in
+  let log:irtext = if mac_log then HS.ref t else () in
+  let a = zero #(alg_of_id i) in
+  Acc #i a log
